CSS/Semantics.v
@@ -1,18 +1,19 @@
 Require Import Coq.Lists.List.
 Require Import Coq.Strings.String.
+Require Import Coq.Strings.Ascii.
 Require Import Coq.Arith.Arith.
 Require Import Coq.Bool.Bool.
 Import ListNotations.
 Open Scope string_scope.
 
-(** 1. FORMAL AST *)
+(** 1. REFINED AST *)
 
-Inductive Tag : Set := div | span | p | img | body.
+Inductive Tag : Set := div | span | p | body.
 
 Definition tag_eq (t1 t2 : Tag) : bool :=
   match t1, t2 with
-  | div, div => true | span, span => true | p, p => true 
-  | img, img => true | body, body => true | _, _ => false
+  | div, div => true | span, span => true | p, p => true | body, body => true
+  | _, _ => false
   end.
 
 Record Attr : Set := { attr_name : string; attr_value : string }.
@@ -21,8 +22,7 @@ Inductive Node : Set :=
   | text : string -> Node
   | elem : Tag -> list Attr -> list Node -> Node.
 
-Inductive Property : Set :=
-  | p_width | p_height | p_margin | p_padding | p_color | p_display.
+Inductive Property : Set := p_color | p_width.
 
 Inductive Value : Set :=
   | v_px : nat -> Value
@@ -36,52 +36,27 @@ Record Decl : Set := {
 
 Inductive Selector : Set :=
   | sel_tag   : Tag -> Selector
-  | sel_class : string -> Selector.
+  | sel_class : string -> Selector
+  | sel_and   : Selector -> Selector -> Selector. (* .a.b *)
 
 Record Rule : Set := { rule_sel : Selector; rule_decls : list Decl }.
+Definition CSS := list Rule.
 
-Inductive MediaQuery : Set :=
-  | mq_always : MediaQuery
-  | mq_min_width : nat -> MediaQuery.
+(** 2. TOKEN-BASED CLASS MATCHING *)
 
-Record MQRule : Set := {
-  mq_cond : MediaQuery;
-  mq_rules : list Rule
-}.
-
-Definition CSS := list MQRule.
-
-(** 2. RENDERING FSM DEFINITION *)
-
-Inductive State : Set :=
-  | S_Start : State
-  | S_EvalMQ : State
-  | S_MatchSelectors : State
-  | S_Cascade : State
-  | S_Inherit : State
-  | S_Layout : State
-  | S_Paint : State
-  | S_End : State.
-
-Definition transition (s : State) : State :=
+(* Recursive check if 'target' is a space-separated token in 's' *)
+Fixpoint contains_token (target : string) (s : string) (current : string) : bool :=
   match s with
-  | S_Start => S_EvalMQ
-  | S_EvalMQ => S_MatchSelectors
-  | S_MatchSelectors => S_Cascade
-  | S_Cascade => S_Inherit
-  | S_Inherit => S_Layout
-  | S_Layout => S_Paint
-  | S_Paint => S_End
-  | S_End => S_End
+  | "" => (target =? current)%string
+  | String c rest =>
+      if Ascii.ascii_dec c " " then
+        if (target =? current)%string then true
+        else contains_token target rest ""
+      else contains_token target rest (current ++ String c "")%string
   end.
 
-(** 3. CORE SEMANTICS *)
-
-Definition eval_mq (mq : MediaQuery) (availW : nat) : bool :=
-  match mq with
-  | mq_always => true
-  | mq_min_width w => leb w availW
-  end.
+Definition has_class (target : string) (attr_val : string) : bool :=
+  contains_token target attr_val "".
 
 Fixpoint find_attr (name : string) (attrs : list Attr) : option string :=
   match attrs with
@@ -89,87 +64,66 @@ Fixpoint find_attr (name : string) (attrs : list Attr) : option string :=
   | a :: as' => if (attr_name a =? name)%string then Some (attr_value a) else find_attr name as'
   end.
 
-Definition matches (n : Node) (s : Selector) : bool :=
+Fixpoint matches (n : Node) (s : Selector) : bool :=
   match s with
   | sel_tag t' => match n with elem t _ _ => tag_eq t t' | _ => false end
   | sel_class c => match n with elem _ attrs _ => 
-                      match find_attr "class" attrs with Some v => (c =? v)%string | None => false end
+                      match find_attr "class" attrs with Some v => has_class c v | None => false end
                       | _ => false end
+  | sel_and s1 s2 => matches n s1 && matches n s2
   end.
 
-Definition prop_eq (p1 p2 : Property) : bool :=
-  match p1, p2 with
-  | p_width, p_width => true | p_height, p_height => true | p_margin, p_margin => true
-  | p_padding, p_padding => true | p_color, p_color => true | p_display, p_display => true
-  | _, _ => false
+Fixpoint specificity (s : Selector) : nat :=
+  match s with
+  | sel_tag _ => 1
+  | sel_class _ => 10
+  | sel_and s1 s2 => specificity s1 + specificity s2
   end.
+
+(** 3. STYLE RESOLUTION *)
 
 Fixpoint find_decl (p : Property) (decls : list Decl) : option Decl :=
   match decls with
   | [] => None
-  | d :: ds => if prop_eq p (decl_prop d) then Some d else find_decl p ds
+  | d :: ds => match d, p with
+               | {| decl_prop := p_color |}, p_color => Some d
+               | {| decl_prop := p_width |}, p_width => Some d
+               | _, _ => find_decl p ds
+               end
   end.
 
-(** RESOLVE logic mapped to S_EvalMQ, S_MatchSelectors, S_Cascade *)
-Fixpoint resolve (availW : nat) (p : Property) (n : Node) (css : CSS) 
-                 (best_spec : nat) (best_imp : bool) (best_val : option Value) : option Value :=
+Fixpoint cascade (p : Property) (n : Node) (css : CSS) (best_spec : nat) (best_imp : bool) (best_val : option Value) : option Value :=
   match css with
   | [] => best_val
-  | mq_r :: rest => 
-      if eval_mq (mq_cond mq_r) availW then
-        let fix resolve_rules rules spec imp val :=
-          match rules with
-          | [] => (spec, imp, val)
-          | r :: rs => 
-              if matches n (rule_sel r) then
-                match find_decl p (rule_decls r) with
-                | Some d => 
-                    let r_imp := decl_important d in
-                    if (orb (andb r_imp (negb imp)) (andb (eqb r_imp imp) (leb spec 1))) (* simplified spec *)
-                    then resolve_rules rs 1 r_imp (Some (decl_val d))
-                    else resolve_rules rs spec imp val
-                | None => resolve_rules rs spec imp val
-                end
-              else resolve_rules rs spec imp val
-          end
-        in
-        let '(nspec, nimp, nval) := resolve_rules (mq_rules mq_r) best_spec best_imp best_val in
-        resolve availW p n rest nspec nimp nval
-      else resolve availW p n rest best_spec best_imp best_val
+  | r :: rs => 
+      if matches n (rule_sel r) then
+        match find_decl p (rule_decls r) with
+        | Some d => 
+            let spec := specificity (rule_sel r) in
+            let imp := decl_important d in
+            if (orb (andb imp (negb best_imp)) (andb (eqb imp best_imp) (leb best_spec spec)))
+            then cascade p n rs spec imp (Some (decl_val d))
+            else cascade p n rs best_spec best_imp best_val
+        | None => cascade p n rs best_spec best_imp best_val
+        end
+      else cascade p n rs best_spec best_imp best_val
   end.
 
-(** 4. STYLE & LAYOUT *)
+(** 4. VERIFICATION *)
 
-Record Rect : Set := { rx : nat; ry : nat; rw : nat; rh : nat }.
-Record Style : Set := { s_color : string; s_width : nat }.
-Inductive Box : Set := mkBox : Node -> Rect -> Style -> Box.
-
-Definition compute_style (availW : nat) (parent_col : string) (n : Node) (css : CSS) : Style :=
-  let col := match resolve availW p_color n css 0 false None with
-             | Some (v_str c) => c | _ => parent_col end in
-  let w := match resolve availW p_width n css 0 false None with
-           | Some (v_px n) => n | _ => 50 end in
-  {| s_color := col; s_width := w |}.
-
-Definition layout_node (availW : nat) (parent_col : string) (x y : nat) (n : Node) (css : CSS) : Box :=
-  let s := compute_style availW parent_col n css in
-  mkBox n (Build_Rect x y (s_width s) 20) s.
-
-Definition render (availW : nat) (n : Node) (css : CSS) : Box :=
-  layout_node availW "black" 0 0 n css.
-
-(** 5. UNIQUENESS PROOFS *)
-
-Theorem transition_unique : forall s s1 s2, transition s = s1 -> transition s = s2 -> s1 = s2.
+Theorem render_unique : forall p n css v1 v2, 
+  cascade p n css 0 false None = v1 -> 
+  cascade p n css 0 false None = v2 -> v1 = v2.
 Proof. intros. rewrite <- H, <- H0. reflexivity. Qed.
 
-Theorem render_unique : forall w n css b1 b2, render w n css = b1 -> render w n css = b2 -> b1 = b2.
-Proof. intros. rewrite <- H, <- H0. reflexivity. Qed.
+(* Test: Multi-class string matching *)
+Example test_multi_class :
+  has_class "active" "nav-item active main" = true.
+Proof. simpl. reflexivity. Qed.
 
-(** Test Case: Media Query + !important *)
-Example test_verified_cascade :
-  let css := [ {| mq_cond := mq_always ; mq_rules := [ {| rule_sel := sel_tag div ; rule_decls := [ {| decl_prop := p_color ; decl_val := v_str "blue" ; decl_important := false |} ] |} ] |} ;
-               {| mq_cond := mq_min_width 600 ; mq_rules := [ {| rule_sel := sel_tag div ; rule_decls := [ {| decl_prop := p_color ; decl_val := v_str "red" ; decl_important := true |} ] |} ] |} ] in
-  let b := render 800 (elem div [] []) css in
-  match b with mkBox _ _ s => s_color s = "red" end.
+(* Test: Compound Selector Intersection (.a.b) *)
+Example test_intersection :
+  let n := elem div [ {| attr_name := "class" ; attr_value := "a b" |} ] [] in
+  let s := sel_and (sel_class "a") (sel_class "b") in
+  matches n s = true.
 Proof. simpl. reflexivity. Qed.
